Added a "SymState" which is a pair of "locs" and "list constraint". Right now the contraints aren't used (or even tracked) but this is the infrastructure and needed alterations to make all necessary functions use SimState instead of just "locs".
Looks like some of my old lemmas remained too - they are probably
useless (really basic) and will disappear when or after the termination
proof is committed.

compcert-1.8/ia32/Peephole.v
@@ -13,7 +13,8 @@ Require Import Mach.
 Require Import Asm.
 Require Import Coq.ZArith.Zbool.
 Require Import PeepholeLocations.
-
+Require Import Coq.Lists.List.
+Require Import Coq.Program.Basics.
 (*
 mov r1 (r2);      -- r1 <- mem_0 r2_0
 add r2 4;         -- r2 <- r2_0 - 4
@@ -90,6 +91,11 @@ Definition sub_f := binOp SymSubF.
 Definition mult_f := binOp SymMultF.
 Definition div_f := binOp SymDivF.
 
+Inductive Constraint : Type :=
+  | ReadMem  : addrmode -> Constraint
+  | WriteMem : addrmode -> Constraint
+  | DivBy    : SymExpr  -> Constraint.
+
 (* to decide equality of symbolic expressions, we need to decide equality of values *)
 Definition val_eq_dec : forall (v1 v2 : val), {v1 = v2} + {v1 <> v2}.
 refine (fun v1 v2 => 
@@ -142,8 +148,21 @@ Defined.
 (* the type of our location store *)
 Definition locs := @LocStore Loc SymExpr Loc_eq.
 
-Notation "a # b" := (lookup b a) (at level 1, only parsing).
-Notation "a # b <- c" := (update b c a) (at level 1, b at next level).
+Inductive SymState :=
+  | SymSt : list Constraint -> locs -> SymState.
+
+Definition symLocs (s : SymState) : locs :=
+  match s with
+  | SymSt _ l => l
+  end.
+
+Definition symSetLoc (l : Loc) (x : SymExpr) (s : SymState) : SymState :=
+  match s with
+  | SymSt c m => SymSt c (update l  x m)
+  end.
+
+Notation "a # b" := (lookup b (symLocs a)) (at level 1, only parsing).
+Notation "a # b <- c" := (symSetLoc b c a) (at level 1, b at next level).
 
 (** the initial state of our symbolic store returns the initial value
     for a given location. This means that no location is initially
@@ -151,8 +170,9 @@ Notation "a # b <- c" := (update b c a) (at level 1, b at next level).
     "foo". Not sure why I have to restate the decision procedure, but
     there it is *)
 Definition initLocs : locs := initLocStore Loc_eq Initial.
+Definition initSymSt : SymState := SymSt nil initLocs.
 
-Definition eval_addrmode (a: addrmode) (l : locs) : option SymExpr :=
+Definition eval_addrmode (a: addrmode) (l : SymState) : option SymExpr :=
   match a with Addrmode base ofs const =>
     match const with
       | inr (id, ofs') => None
@@ -174,14 +194,14 @@ Definition eval_addrmode (a: addrmode) (l : locs) : option SymExpr :=
 
 Definition symUndef := Imm Vundef.
 
-Definition setAllFlags (l : locs) (e : SymExpr) : locs :=
+Definition setAllFlags (l : SymState) (e : SymExpr) : SymState :=
   l # (Register (CR ZF)) <- e
     # (Register (CR CF)) <- e
     # (Register (CR PF)) <- e
     # (Register (CR SOF)) <- e.
 
 (* small step symbolic execution *)
-Definition single_symExec (i : instruction) (l : locs) : option locs :=
+Definition single_symExec (i : instruction) (l : SymState) : option SymState :=
   match i with
   | Pnop => Some l
       (** Moves *)
@@ -462,7 +482,7 @@ Definition single_symExec (i : instruction) (l : locs) : option locs :=
   end.
 
 
-Fixpoint symExec (c : code) (l : locs) : option locs :=
+Fixpoint symExec (c : code) (l : SymState) : option SymState :=
   match c with
     | nil => Some l
     | i :: is => match (single_symExec i l) with
@@ -479,7 +499,7 @@ Notation "a '&&&' b" :=
     else Utils.in_right).
 
 
-Fixpoint allLocs_dec (l : list Loc) (a b : locs) : bool :=
+Fixpoint allLocs_dec (l : list Loc) (a b : SymState) : bool :=
   match l with
     | nil => true
     | l' :: ls => 
@@ -500,14 +520,14 @@ Fixpoint all {A : Type} (p : A -> bool) (xs : list A) : bool :=
     | _   => false
   end.
 
-Definition validFlags (x : list Loc) (c : locs) (d : locs) : bool := 
+Definition validFlags (x : list Loc) (c : SymState) (d : SymState) : bool := 
   all (fun l => SymExpr_dec (c # l) symUndef || SymExpr_dec (c # l) (d # l)) x.
 
-Definition sameSymbolicExecution (c : option locs) (d : option locs) : bool :=
+Definition sameSymbolicExecution (c : option SymState) (d : option SymState) : bool :=
   match c, d with
     | Some c', Some d' =>
-      let (flagC, nonFlagC) := partition (fun x => isCR x) (elements c') in
-        let (flagD, nonFlagD) := partition (fun x => isCR x) (elements d') in
+      let (flagC, nonFlagC) := partition (fun x => isCR x) (elements (symLocs c')) in
+        let (flagD, nonFlagD) := partition (fun x => isCR x) (elements (symLocs d')) in
           allLocs_dec (nonFlagC ++ nonFlagD) c' d' && validFlags (flagC ++ flagD) c' d'
     | _, _ => false
   end.
@@ -519,9 +539,9 @@ Definition sameSymbolicExecution (c : option locs) (d : option locs) : bool :=
   doesn't return false given certain known-correct conditions, but
   that isn't required.
  *)
-Fixpoint peephole_validate (c : Asm.code) (d : Asm.code) (l : locs) : bool :=
+Fixpoint peephole_validate (c : Asm.code) (d : Asm.code) : bool :=
   if (negb (beq_nat (length c) 0)) && Compare_dec.leb (length d) (length c)
-    then sameSymbolicExecution (symExec c l) (symExec d l)    
+    then sameSymbolicExecution (symExec c initSymSt) (symExec d initSymSt)    
     else false.
 
 Parameter ml_optimize : Asm.code -> Asm.code.
@@ -532,7 +552,7 @@ Parameter ml_optimize : Asm.code -> Asm.code.
   used, otherwise, they are discarded. **)
 Definition opt_window (c : Asm.code) :=
   let c' := ml_optimize c
-  in if peephole_validate c c' initLocs
+  in if peephole_validate c c'
       then c'
       else c.
 
@@ -551,10 +571,10 @@ Proof.
   simpl. remember (Compare_dec.leb (length (ml_optimize (i :: c)))
                  (Datatypes.S (length c))) as len.
   destruct len. remember (sameSymbolicExecution
-              match single_symExec i initLocs with
+              match single_symExec i initSymSt with
               | Some l' => symExec c l'
               | None => None
-              end (symExec (ml_optimize (i :: c)) initLocs)) as ssE.
+              end (symExec (ml_optimize (i :: c)) initSymSt)) as ssE.
   destruct ssE. assumption. simpl. apply leb_n_n_true. simpl. apply leb_n_n_true.
 Qed.
 
@@ -581,7 +601,7 @@ Qed.
 Fixpoint only_opt_instrs (c : code) : code :=
   match c with 
     | nil => nil
-    | x :: xs => match (single_symExec x initLocs) with
+    | x :: xs => match (single_symExec x initSymSt) with
                    | None => nil
                    | Some _ => x :: only_opt_instrs xs 
                  end
@@ -590,40 +610,38 @@ Fixpoint only_opt_instrs (c : code) : code :=
 Function basic_block (c : Asm.code) {measure length c} : list Asm.code :=
   match c with
     | nil => nil
-    | x :: xs => match (single_symExec x initLocs) with
+    | x :: xs => match (single_symExec x initSymSt) with
                    | None => (x :: nil) :: nil (* singleton of unoptimized instr *)
                    | Some _ => let opts := only_opt_instrs xs 
                      in (x :: opts) :: basic_block (skipn (length opts) xs)
                  end
   end. intros. simpl. auto.
+Admitted.
 
-Fixpoint partitionSymExec (c : Asm.code) : list Asm.code :=
-  match c with
-    | nil => nil
-    | x :: xs => match single_symExec x initLocs with
-                   | None => (x :: nil)
-                   | 
+Definition concat (c : list Asm.code) : Asm.code := fold_left (fun a b => a ++ b) c nil.
+
+Definition optimize (c : Asm.code) : Asm.code :=
+  let parts := basic_block c in concat parts. (* (map opt_window parts). *)
 
 Fixpoint partitionSymExec (c : Asm.code) : (Asm.code * Asm.code) :=
   match c with
     | nil     => (pair nil nil)
-    | (x::xs) => match single_symExec x initLocs with
+    | (x::xs) => match single_symExec x initSymSt with
                    | None => pair nil (x::xs)
                    | _    => let (cs,bs) := partitionSymExec xs in pair (x::cs) bs
                      end
     end.
 
-Function optimize (c : Asm.code) {measure length c} : Asm.code :=
+
+Function optimize2 (c : Asm.code) {measure length c} : Asm.code :=
   let part := partitionSymExec c in
     let len := length (fst part) in
       match snd part with
         | nil     => opt_window (fst part)
-        | (r::rs) => opt_window (fst part) ++ optimize (r::skipn (len + 1) c)
-    end. intros.
-    destruct (fst (partitionSymExec c)).
-    simpl.  destruct c. inversion teq.
+        | (r::rs) => opt_window (fst part) ++ optimize2 (r::skipn (len + 1) c)
+    end.
+Admitted.
     
-
 Definition transf_function (f: Asm.code) : res Asm.code :=
   OK (optimize f).
 
